
\item Match fails:
\begin{itemize}[leftmargin=\secondm]
   \item $s_2 = \derstatex{\Gamma}{\Delta_N}{\Xi}{\Gamma_{N1}}{\Delta_{N1}}
{(\lambda x.  C\{\Psi(\widehat{v})/\widehat{v}\} x) \Sigma,
   \Omega_N}$
\end{itemize}

\item Match succeeds with backtracking to a linear continuation frame in
stack $\lstack{C}$ ($\lstack{C} \neq \cdot$):

\begin{itemize}[leftmargin=\secondm]
   \item $s_2 = \matstatea{\Delta_N}{\lstack{C'''}, f', \lstack{C''};
                  \lstack{P}}{\Gamma}{\Delta_c}{\cdot}
               {\Delta'_f, p_2, \Delta'' \rightarrow \Omega_f \otimes p
                  \otimes split(\Omega'_f)}{\Sigma}$

   \item $\lstack{C} = \lstack{C'}, f, \lstack{C''}$
   \item $f = \lframe{\Delta_a}{\Delta_{b_1}, p_2,
         \Delta_{b_2}}{p}{\Omega_f}{\Delta_f'}{\Omega'_f}$
         turns into
         $f' = \lframe{\Delta_a, \Delta_{b_1}, p_2}
            {\Delta_{b_2}}{p}{\Omega_f}{\Delta'_f}{\Omega'_f}$
   %\item $\Delta_c = (\Delta_1, \Delta_2, \Delta') - (\Delta'_f, \Delta'', p_2)$
\end{itemize}

\item Match succeeds with backtracking to a persistent continuation frame
in stack $\lstack{C}$ ($\lstack{C} \neq \cdot$):
\begin{itemize}[leftmargin=\secondm]
   \item $s_2 = \matstatea{\Delta_N}{\lstack{C'''}, f', \lstack{C''};
      \lstack{P}}{\Gamma}{\Delta_{c_1}}{\cdot}{\Delta'_f, \Delta_{c_2}, 
         \rightarrow \Omega_f \otimes \bang p \otimes split(\Omega'_f)}{\Sigma}$

   \item $\lstack{C} = \lstack{C'}, f, \lstack{C''}$

   \item $f = \pframe{\Gamma_1, p_2,
      \Gamma_2}{\Delta_{c_1}, \Delta_{c_2}}{\bang p}{\Omega_f}{\Delta'_f}{\Omega'_f}$
   turns into $f' = \pframe{\Gamma_2}{\Delta_{c_1},
      \Delta_{c_2}}{\bang p}{\Omega_f}{\Delta'_f}{\Omega'_f}$

   %\item $\Delta_{c_1}, \Delta_{c_2} = (\Delta_1, \Delta_2,
   %      \Delta') - \Delta'_f$
\end{itemize}

\item Match succeeds with backtracking to a persistent continuation frame
in stack $\lstack{P}$ ($\lstack{C} = \cdot$):
\begin{itemize}[leftmargin=\secondm]
   \item $s_2 = \matstatea{\Delta_N}{\lstack{C'}; \lstack{P'''}, f', \lstack{P''}}
         {\Gamma}{\Delta_{c_1}}{\cdot}{\Delta'_f, \Delta_{c_2}, 
         \rightarrow \Omega_f \otimes \bang p \otimes split(\Omega'_f)}{\Sigma}$

   \item $\lstack{P} = \lstack{P'}, f, \lstack{P''}$

   \item $f = \pframe{\Gamma_1, p_2,
      \Gamma_2}{\Delta_{c_1}, \Delta_{c_2}}{\bang p}{\Omega_f}{\Delta'_f}{\Omega'_f}$
   turns into $f' = \pframe{\Gamma_2}{\Delta_{c_1},
      \Delta_{c_2}}{\bang p}{\Omega_f}{\Delta'_f}{\Omega'_f}$

   %\item $\Delta_{c_1}, \Delta_{c_2} = (\Delta_1, \Delta_2,
   %      \Delta') - \Delta'_f$
\end{itemize}
